add hash-map to proofs/

proofs/impls/hash-map.bpl
@@ -2,7 +2,8 @@
 // A simplified hash table implementation with weakly consistent contains method.
 //
 // Compared to Java's hash map, we assume:
-// - The hash function is identity
+// - The hash function is assumed to be injective for simplicity,
+// otherwise one needs to have lists at each bucket to deal with hash collisions
 // - Each bucket stores a single value as opposed to a list
 // - There is no resizing of the hash table
 //
@@ -17,6 +18,14 @@ var {:layer 0,1} table: [int]int;
 const tabLen: int;
 axiom 0 < tabLen;
 
+// The hash function
+function hash(k: int) : int;
+axiom (forall k: int :: 0 <= hash(k) && hash(k) < tabLen);
+// Assume the hash function is injective, for simplicity
+axiom (forall k1, k2: int :: hash(k1) == hash(k2) ==> k1 == k2);
+function hash_inv(i: int) : int;
+axiom (forall i: int :: {hash(hash_inv(i))} hash(hash_inv(i)) == i);
+
 // Visibility per location of concrete state
 var {:layer 1,1} tabvis: [int]SetInvoc;
 
@@ -27,7 +36,6 @@ var {:layer 1,1} called: [Invoc]bool;
 // The set of invocations that have returned
 var {:layer 1,1} returned: [Invoc]bool;
 
-
 // The invariants
 function {:inline} tableInv(table: [int]int, tabvis: [int]SetInvoc,
                             hb: [Invoc][Invoc]bool, lin: SeqInvoc, vis: [Invoc]SetInvoc, tabLen: int,
@@ -36,15 +44,15 @@ function {:inline} tableInv(table: [int]int, tabvis: [int]SetInvoc,
   // tabvis only contains linearized things
   (forall i: int :: 0 <= i && i < tabLen
     ==> Set_subset(tabvis[i], Set_ofSeq(lin)))
-  // tabvis[i] contains everything in lin of key i
-  && (forall i: int :: 0 <= i && i < tabLen
-    ==> Set_subset(Map.restr(Set_ofSeq(lin), i), tabvis[i]))
-  // tabvis[i] only has puts to key k
+  // tabvis[i] contains everything in lin of keys that hash to i
+  && (forall k: int :: 0 <= hash(k) && hash(k) < tabLen
+    ==> Set_subset(Map.restr(Set_ofSeq(lin), k), tabvis[hash(k)]))
+  // tabvis[i] only has puts to keys that hash to i
   && (forall i: int, n: Invoc :: 0 <= i && i < tabLen && tabvis[i][n]
-    ==> invoc_m(n) == Map.put && invoc_k(n) == i)
-  // lin|tabvis[i] gives value of key i
-  && (forall i: int :: 0 <= i && i < tabLen
-    ==> Map.ofSeq(Seq_restr(lin, tabvis[i]))[i] == table[i])
+    ==> invoc_m(n) == Map.put && hash(invoc_k(n)) == i)
+  // lin|tabvis[i] gives value of keys that hash to i
+  && (forall k: int ::
+    Map.ofSeq(Seq_restr(lin, tabvis[hash(k)]))[k] == table[hash(k)])
 
   // ---- Invariants of the specification program:
   // lin only contains called things
@@ -59,6 +67,32 @@ function {:inline} tableInv(table: [int]int, tabvis: [int]SetInvoc,
   // To establish precondition of intro_writeLin
   && (forall n: Invoc :: returned[n] ==> Seq_elem(n, lin))
 }
+
+  // // tabvis only contains linearized things
+  // assert {:layer 1} (forall i: int :: 0 <= i && i < tabLen
+  //   ==> Set_subset(tabvis[i], Set_ofSeq(lin)));
+  // // tabvis[i] contains everything in lin of keys that hash to i
+  // assert {:layer 1} (forall k1: int :: 0 <= hash(k1) && hash(k1) < tabLen
+  //   ==> Set_subset(Map.restr(Set_ofSeq(lin), k1), tabvis[hash(k1)]));
+  // // tabvis[i] only has puts to keys that hash to i
+  // assert {:layer 1} (forall i: int, n: Invoc :: 0 <= i && i < tabLen && tabvis[i][n]
+  //   ==> invoc_m(n) == Map.put && hash(invoc_k(n)) == i);
+  // // lin|tabvis[i] gives value of keys that hash to i
+  // assert {:layer 1} (forall k1: int ::
+  //   Map.ofSeq(Seq_restr(lin, tabvis[hash(k1)]))[k1] == table[hash(k1)]);
+
+  // // ---- Invariants of the specification program:
+  // // lin only contains called things
+  // assert {:layer 1} (forall n: Invoc :: {Seq_elem(n, lin)} Seq_elem(n, lin) ==> called[n]);
+  // // lin contains distinct elements
+  // assert {:layer 1} Seq_distinct(lin);
+  // // vis sets only contain linearized ops
+  // assert {:layer 1} (forall n1, n2: Invoc :: {vis[n2][n1]}
+  //   vis[n2][n1] && returned[n2] ==> Set_ofSeq(lin)[n1]);
+  // // Used to infer that invocations don't modify vis after they've returned
+  // assert {:layer 1} (forall n1, n2 : Invoc :: called[n1] && hb[n2][n1] ==> returned[n2]);
+  // // To establish precondition of intro_writeLin
+  // assert {:layer 1} (forall n: Invoc :: returned[n] ==> Seq_elem(n, lin)) ;
 
 function {:inline} preLP(called: [Invoc]bool, returned: [Invoc]bool, lin: SeqInvoc, this: Invoc) : bool
 {
@@ -94,17 +128,17 @@ procedure {:yields} {:layer 0} {:refines "readTable_atomic"} readTable(k: int)
 
 // ---------- Primitives for manipulating logical/abstract state
 
-procedure {:layer 1} intro_add_tabvis(k: int, n: Invoc)
-  ensures {:layer 1} tabvis == old(tabvis)[k := Set_add(old(tabvis)[k], n)];
+procedure {:layer 1} intro_add_tabvis(i: int, n: Invoc)
+  ensures {:layer 1} tabvis == old(tabvis)[i := Set_add(old(tabvis)[i], n)];
   modifies tabvis;
 {
-  tabvis[k] := Set_add(tabvis[k], n);
+  tabvis[i] := Set_add(tabvis[i], n);
 }
 
-procedure {:layer 1} intro_read_tabvis(k: int) returns (s: SetInvoc)
-  ensures {:layer 1} s == tabvis[k];
+procedure {:layer 1} intro_read_tabvis(i: int) returns (s: SetInvoc)
+  ensures {:layer 1} s == tabvis[i];
 {
-  s := tabvis[k];
+  s := tabvis[i];
 }
 
 procedure {:layer 1} {:inline 1} intro_writeCalled({:linear "this"} this: Invoc)
@@ -150,7 +184,6 @@ procedure {:yields} {:layer 1} {:refines "put_call_atomic"}
   assert {:layer 1} preLP(called, returned, lin, this);
 }
 
-
 procedure {:yields} {:layer 1} {:refines "put_atomic"} put(k, v: int, {:linear "this"} this: Invoc)
   requires {:layer 1} tableInv(table, tabvis, hb, lin, vis, tabLen, called, returned);
   requires {:layer 1} preLP(called, returned, lin, this);
@@ -164,9 +197,9 @@ procedure {:yields} {:layer 1} {:refines "put_atomic"} put(k, v: int, {:linear "
   var {:layer 1} my_vis: SetInvoc;
   yield; assert {:layer 1} tableInv(table, tabvis, hb, lin, vis, tabLen, called, returned) && preLP(called, returned, lin, this);
 
-  call writeTable(k, v);
+  call writeTable(hash(k), v);
 
-  call intro_add_tabvis(k, this);
+  call intro_add_tabvis(hash(k), this);
   call my_vis := intro_readLin();
   call intro_writeLin(this);
   call intro_writeVis(this, my_vis);
@@ -225,7 +258,7 @@ procedure {:yields} {:layer 1} {:refines "get_atomic"} get(k: int, {:linear "thi
   var {:layer 1} my_vis: SetInvoc;
   yield; assert {:layer 1} tableInv(table, tabvis, hb, lin, vis, tabLen, called, returned) && preLP(called, returned, lin, this);
 
-  call v := readTable(k);
+  call v := readTable(hash(k));
 
   call my_vis := intro_readLin();
   call intro_writeVis(this, my_vis);
@@ -253,7 +286,6 @@ procedure {:yields} {:layer 1} {:refines "get_return_atomic"}
   assert {:layer 1} tableInv(table, tabvis, hb, lin, vis, tabLen, called, returned);
 }
 
-
 procedure {:yields} {:layer 1} {:refines "contains_call_atomic"}
     contains_call({:linear "this"} this: Invoc)
   requires {:layer 1} tableInv(table, tabvis, hb, lin, vis, tabLen, called, returned);
@@ -272,6 +304,9 @@ procedure {:yields} {:layer 1} {:refines "contains_call_atomic"}
   assert {:layer 1} preLP(called, returned, lin, this);
 }
 
+procedure {:layer 1} assume_false();
+  ensures {:layer 1} false;
+
 procedure {:yields} {:layer 1} {:refines "contains_atomic"}
     contains(v: int, {:linear "this"} this: Invoc)
   returns (res: bool, witness_k: int)
@@ -283,50 +318,53 @@ procedure {:yields} {:layer 1} {:refines "contains_atomic"}
   ensures {:layer 1} (forall n1: Invoc :: {vis[this][n1]}
     vis[this][n1] ==> Set_ofSeq(lin)[n1]);
 {
-  var k, tv: int;
+  var i, tv: int;
   var {:layer 1} my_vis, my_vis1: SetInvoc;
   yield;
   assert {:layer 1} tableInv(table, tabvis, hb, lin, vis, tabLen, called, returned) && preLP(called, returned, lin, this);
 
-  k := 0;
+  i := 0;
   call my_vis := intro_readLin();
   yield;
   assert {:layer 1} tableInv(table, tabvis, hb, lin, vis, tabLen, called, returned) && preLP(called, returned, lin, this);
-  assert {:layer 1} (forall j: Invoc :: hb[j][this] ==> Set_subset(vis[j], my_vis));
+  assert {:layer 1} (forall j: Invoc :: hb[j][this]
+    ==> Set_subset(vis[j], my_vis));
   assert {:layer 1} (forall n1: Invoc :: {my_vis[n1]}
     my_vis[n1] ==> Set_ofSeq(lin)[n1]);
-  assert {:layer 1} (forall i: int :: 0 <= i && i < tabLen
-    ==> Set_subset(Map.restr(my_vis, i), tabvis[i]));
+  assert {:layer 1} (forall k1: int ::
+    Set_subset(Map.restr(my_vis, k1), tabvis[hash(k1)]));
 
-  while (k < tabLen)
-    invariant {:layer 1} 0 <= k && k <= tabLen;
+  while (i < tabLen)
+    invariant {:layer 1} 0 <= i && i <= tabLen;
     invariant {:layer 1} tableInv(table, tabvis, hb, lin, vis, tabLen, called, returned) && preLP(called, returned, lin, this);
-    invariant {:layer 1} (forall i: int :: 0 <= i && i < k
-      ==> Map.ofSeq(Seq_restr(lin, my_vis))[i] != v);
-    invariant {:layer 1} (forall j: Invoc :: hb[j][this] ==> Set_subset(vis[j], my_vis));
+    invariant {:layer 1} (forall k: int :: 0 <= hash(k) && hash(k) < i
+      ==> Map.ofSeq(Seq_restr(lin, my_vis))[k] != v);
+    invariant {:layer 1} (forall j: Invoc :: hb[j][this]
+      ==> Set_subset(vis[j], my_vis));
     invariant {:layer 1} (forall n1: Invoc :: {my_vis[n1]}
       my_vis[n1] ==> Set_ofSeq(lin)[n1]);
-    invariant {:layer 1} (forall i: int :: 0 <= i && i < tabLen
-      ==> Set_subset(Map.restr(my_vis, i), tabvis[i]));
+    invariant {:layer 1} (forall k1: int ::
+      Set_subset(Map.restr(my_vis, k1), tabvis[hash(k1)]));
   {
-    // Read table[k] and add tabvis[k] to my_vis
-    call tv := readTable(k);
+    // Read table[i] and add tabvis[i] to my_vis
+    call tv := readTable(i);
 
-    call my_vis1 := intro_read_tabvis(k);
+    call my_vis1 := intro_read_tabvis(i);
     my_vis := Set_union(my_vis, my_vis1);
 
-    assert {:layer 1} Map.restr(my_vis, k) == Map.restr(tabvis[k], k);
-    assert {:layer 1} Map.ofSeq(Seq_restr(lin, tabvis[k]))[k]
-      == Map.ofSeq(Seq_restr(lin, Map.restr(tabvis[k], k)))[k];
+    assert {:layer 1} Map.restr(my_vis, hash_inv(i)) == Map.restr(tabvis[i], hash_inv(i));
+    assert {:layer 1} Map.ofSeq(Seq_restr(lin, tabvis[i]))[i]
+      == Map.ofSeq(Seq_restr(lin, Map.restr(tabvis[i], i)))[i];
 
-    assert {:layer 1} (forall i: int :: 0 <= i && i < k
-      ==> Map.ofSeq(Seq_restr(lin, my_vis))[i] == Map.ofSeq(Seq_restr(lin, Map.restr(my_vis, i)))[i]);
+    assert {:layer 1} (forall k: int :: 0 <= hash(k) && hash(k) < i
+      ==> Map.ofSeq(Seq_restr(lin, my_vis))[k] 
+        == Map.ofSeq(Seq_restr(lin, Map.restr(my_vis, k)))[k]);
 
     if (tv == v) {
       // Linearization point
       call intro_writeVis(this, my_vis);
       call intro_writeLin(this);
-      witness_k := k;
+      witness_k := hash_inv(i);
 
       res := true;
 
@@ -337,21 +375,21 @@ procedure {:yields} {:layer 1} {:refines "contains_atomic"}
         vis[this][n1] ==> Set_ofSeq(lin)[n1]);
       return;
     }
-    k := k + 1;
+    i := i + 1;
     yield;
     assert {:layer 1} tableInv(table, tabvis, hb, lin, vis, tabLen, called, returned) && preLP(called, returned, lin, this);
-    assert {:layer 1} (forall i: int :: 0 <= i && i < k
-      ==> Map.ofSeq(Seq_restr(lin, my_vis))[i] != v);
+    assert {:layer 1} (forall k: int :: 0 <= hash(k) && hash(k) < i
+      ==> Map.ofSeq(Seq_restr(lin, my_vis))[k] != v);
     assert {:layer 1} (forall j: Invoc :: hb[j][this] ==> Set_subset(vis[j], my_vis));
     assert {:layer 1} (forall n1: Invoc :: {my_vis[n1]}
       my_vis[n1] ==> Set_ofSeq(lin)[n1]);
-    assert {:layer 1} (forall i: int :: 0 <= i && i < tabLen
-      ==> Set_subset(Map.restr(my_vis, i), tabvis[i]));
+    assert {:layer 1} (forall k1: int ::
+      Set_subset(Map.restr(my_vis, k1), tabvis[hash(k1)]));
   }
   yield;
   assert {:layer 1} tableInv(table, tabvis, hb, lin, vis, tabLen, called, returned) && preLP(called, returned, lin, this);
-  assert {:layer 1} (forall i: int :: 0 <= i && i < tabLen
-    ==> Map.ofSeq(Seq_restr(lin, my_vis))[i] != v);
+  assert {:layer 1} (forall k: int :: 0 <= hash(k) && hash(k) < i
+    ==> Map.ofSeq(Seq_restr(lin, my_vis))[k] != v);
   assert {:layer 1} (forall j: Invoc :: hb[j][this] ==> Set_subset(vis[j], my_vis));
   assert {:layer 1} (forall n1: Invoc :: {my_vis[n1]}
     my_vis[n1] ==> Set_ofSeq(lin)[n1]);
@@ -359,11 +397,11 @@ procedure {:yields} {:layer 1} {:refines "contains_atomic"}
   // Linearization point
   call intro_writeVis(this, my_vis);
   call intro_writeLin(this);
-  witness_k := k;
 
   res := false;
 
   call intro_writeRet(this, RetVal_ofBool(res));
+
   yield; assert {:layer 1} tableInv(table, tabvis, hb, lin, vis, tabLen, called, returned)
     && postLP(called, returned, lin, this);
   assert {:layer 1} (forall n1: Invoc :: {vis[this][n1]}
